fixing files after modifying LambdaRef.v

src/Aux.v
@@ -21,15 +21,15 @@ Proof.
       * now apply IHl.
 Qed.
 
-Definition get_fresh {V : Set} (m : Map V) : Label :=
+Definition get_fresh (m : Map) : Label :=
   OfNat (1 + list_max (List.map (fun '(OfNat n) => n) (labels m))).
 
 Lemma map_lt_get_fresh :
-  forall (V : Set) (m : Map V) (M : nat),
+  forall (m : Map) (M : nat),
     OfNat M = get_fresh m ->
     List.Forall (fun '(OfNat x) => x < M) (labels m).
 Proof.
-  intros ? ? ? HM. unfold get_fresh in HM. simpl in HM.
+  intros ? ? HM. unfold get_fresh in HM. simpl in HM.
   injection HM as HM.
   match goal with
   | [H : M = S (list_max ?l) |- _] =>
@@ -45,7 +45,7 @@ Proof.
 Qed.
 
 Lemma map_neq_get_fresh :
-  forall (V : Set) (m : Map V),
+  forall (m : Map),
     List.Forall (fun l => l <> get_fresh m) (labels m).
 Proof.
   intros. destruct (get_fresh m) as [M] eqn:Hfresh.
@@ -55,9 +55,9 @@ Proof.
   - now apply map_lt_get_fresh.
 Qed.
 
-Lemma has_fresh : forall V (m : Map V), Is_fresh_label (get_fresh m) m.
+Lemma has_fresh : forall (m : Map), Is_fresh_label (get_fresh m) m.
 Proof.
-  unfold Is_fresh_label. intros ? ? HIn.
+  unfold Is_fresh_label. intros ? HIn.
   apply -> List.Forall_forall in HIn.
   2: apply map_neq_get_fresh.
   now simpl in HIn.
