src/Tactics.v
@@ -1,11 +1,5 @@
 Require Import src.LambdaRef.
 
-Ltac solve_typing :=
-  repeat econstructor; simpl;
-  match goal with
-  | [ |- T[ ?G |- Val (Var ?x) ::: ?t ] ] => apply (T_Var G x)
-  end.
-
 Ltac solve_cost_red x :=
   repeat (eapply no_red || (eapply S_red; [ x | ])).
 
